saving before Australia trip

Attest/appJ/appraiser/compilation/.#appraiserCompileScript.sml
@@ -1,0 +1,1 @@
+guardol@guardol-host.7500:1572373311
