Attest/appJ/appraiser/compilation/appraiserCompileScript.sml
@@ -1,0 +1,31 @@
+(*
+  Compile appraiser program the quick-and-dirty way with the
+  unverified S-expression bootstrap. Assumes a cake binary on
+  your $PATH
+ *)
+open bossLib preamble ml_progLib ml_translatorLib;
+open appraiserTheory fromSexpTheory;
+open astToSexprLib;
+
+
+val _ = new_theory "appraiserCompile";
+
+val _ = translation_extends "appraiser";
+
+(* Convert the list of declarations comprising the appraiser from SNOC list to CONS list *)
+val appraiser_prog = get_ml_prog_state() |> get_prog |> EVAL |> concl |> rhs;
+
+(* Pretty-print aforementioned CONS list as an s-expression *)
+val _ = write_ast_to_file "appraiser.sexp" appraiser_prog;
+
+(* In terminal:
+
+ > cake --skip_type_inference=true --sexp=true < appraiser.sexp > appraiser.S
+
+  To link:
+
+ > gcc appraiser.S $CAKEMLDIR/basis/basis_ffi.c -o appraiser
+
+ *)
+
+val _ = export_theory();
