Attest/appJ/appraiser/compilation/appraiserEvalCompileScript.sml
@@ -1,0 +1,31 @@
+(*
+  Compile appraiser program the nice-and-slow way by evaluating
+  the CakeML compiler in-logic.
+ *)
+open bossLib preamble ml_progLib ml_translatorLib;
+open appraiserTheory;
+open compilationLib;
+
+
+val _ = new_theory "appraiserEvalCompile";
+
+val _ = translation_extends "appraiser";
+
+(* Convert the list of declarations comprising the appraiser from SNOC list to CONS list.
+   Save in a def becase compile_x64 expects a thm where the rhs is the prog in question *)
+Definition appraiser_prog_def:
+  appraiser_prog = ^(get_ml_prog_state() |> get_prog |> EVAL |> concl |> rhs)
+End
+
+(* Compile, export the resulting ELF template to a file,
+   and produce a theorem certifying that the machine code therein is the
+   compiler output *)
+val compile_thm = compile_x64 1000 1000 "eval_appraiser" appraiser_prog_def
+
+(* In terminal:
+
+ > gcc eval_appraiser.S $CAKEMLDIR/basis/basis_ffi.c -o appraiser
+
+ *)
+
+val _ = export_theory();
