Attest/appJ/appraiser/coplandScript.sml
@@ -1,0 +1,93 @@
+open HolKernel boolLib Parse bossLib;
+open stringLib;
+open finite_mapLib;
+
+open preamble
+open ml_translatorTheory;
+open ml_translatorLib ml_progLib;
+open basisFunctionsLib;
+open basisProgTheory;
+open wordsTheory;
+open comparisonTheory;
+
+val _ = new_theory "copland";
+
+(*---------------------------------------------------------------------------*)
+(* Terms                                                                     *)
+(*---------------------------------------------------------------------------*)
+val res = type_abbrev ("place",``:word32``);
+val res = type_abbrev ("mid",  ``:num``);
+val res = type_abbrev("pi", ``:bool # bool``); (* provisional *)
+
+(* Explicitly typed w2n to word32 to avoid running into problems with dimindex/the 'itself' constructor *)
+val w322n_def = Define `w322n (w:word32) = w2n w`;
+
+val place_cmp_def = Define
+  `place_cmp (p1 : place) (p2 : place) = num_cmp (w322n p1) (w322n p2)`;
+
+val res = translate num_cmp_def;
+val res = translate w322n_def;
+val res = translate place_cmp_def;
+
+val _ = Hol_datatype
+  `term = USM of mid => string list  (* User space measurement *)
+        | KIM of mid => place => string list (* Kernel integrity measurement *)
+	      | SIG
+	      | HSH
+	      | CPY
+	      | NONCE
+        | AT of place => term
+        | LN of term => term
+        | BRS of pi => term => term
+        | BRP of pi => term => term`;
+
+val _ = Hol_datatype
+  `evidence (* akin to values in a PL *) (* more like types. They're abstract versions of the concrete evidence below *)
+       = Mt
+       | U of place => evidence  (* User space measurement evidence *)
+       | K of place => place => evidence
+       | G of evidence => place
+       | H of evidence => place
+       | N of place => evidence
+       | SS of evidence => evidence
+       | PP of evidence => evidence`;
+
+
+(*---------------------------------------------------------------------------*)
+(* Concrete Evidence                                                         *)
+(*---------------------------------------------------------------------------*)
+
+val res = type_abbrev ("args",``:string list``);
+val res = type_abbrev ("bits", ``:string``); (* base64 (or 16 now?) encoded string *)
+
+val _ = Hol_datatype
+  `concrete
+       = MT
+       | CUSM of place => mid => args => bits => concrete  (* User space measurement concrete *)
+       | CKSM of place => place => mid => args => bits => concrete
+       | CSIG of place => concrete => bits
+       | CHASH of place => bits
+       | CNONCE of place => bits => concrete
+       | CSEQ of concrete => concrete
+       | CPAR of concrete => concrete`;
+
+(*---------------------------------------------------------------------------*)
+(* Messages                                                                  *)
+(*---------------------------------------------------------------------------*)
+
+val res = type_abbrev ("address",``:num``);
+
+val _ = Hol_datatype
+   `request = <| toPlace : place ;
+                 fromPlace : place ;
+		             reqNameMap : place |-> address ;
+		             reqTerm : term ;
+		             reqEv : concrete |>`;
+
+
+val _ = Hol_datatype
+  `response = <| respToPlace : place ;
+                 respFromPlace : place ;
+		             respEv : concrete |>`;
+
+val _ = export_theory();
