Attest/appraiser/appraiserScript.sml
@@ -1,0 +1,157 @@
+open HolKernel Parse boolLib bossLib;
+open preamble semanticPrimitivesTheory;
+open ml_translatorTheory;
+open ml_translatorLib;
+open ml_monad_translator_interfaceLib;
+open ml_progLib;
+open MapProgTheory;
+open basisFunctionsLib;
+open basisProgTheory;
+
+open balanced_mapTheory;
+open coplandTheory;
+open comparisonTheory;
+open wordsTheory;
+
+val _ = new_theory "appraiser";
+val _ = numLib.prefer_num ();
+
+val sel4AM_def     = Define `sel4AM = 1w : place`;
+val platformAM_def = Define `platformAM = 2w : place`;
+val userAM_def     = Define `userAM = 3w : place`;
+
+val usm11_def = Define `usm11 = 11`;
+val kim11_def = Define `kim21 = 21`;
+
+val attestation_cmd_def = Define
+    `attestation_cmd = LN (AT platformAM (LN (AT sel4AM (LN (KIM kim21 platformAM [])
+                                                            SIG))
+                                             (LN (KIM kim21 userAM []) SIG)))
+                          (LN (USM usm11 []) SIG)`;
+
+val expected_bs1_def = Define `expected_bs1 = "1234"`;
+val expected_bs2_def = Define `expected_bs2 = "2234"`;
+val expected_bs3_def = Define `expected_bs3 = "3234"`;
+val expected_bs4_def = Define `expected_bs4 = "4234"`;
+val expected_bs5_def = Define `expected_bs5 = "5234"`;
+val expected_bs6_def = Define `expected_bs6 = "6234"`;
+
+val appraise_def = Define
+    `(appraise (CSIG uAM (CUSM uAM2 u [] b5
+                   (CSIG pAM (CKSM pAM2 uAM3 k1 [] b3
+                       (CSIG sAM (CKSM sAM2 pAM3 k2 [] b1 MT) b2))
+                       b4))
+                   b6)
+       = ((b6 = expected_bs6) /\ (b5 = expected_bs5) /\
+          (b4 = expected_bs4) /\ (b3 = expected_bs3) /\
+          (b2 = expected_bs2) /\ (b1 = expected_bs1) /\
+          (uAM = userAM)      /\ (uAM2 = userAM)     /\ (uAM3 = userAM)     /\
+          (pAM = platformAM)  /\ (pAM2 = platformAM) /\ (pAM3 = platformAM) /\
+          (sAM = sel4AM)      /\ (sAM2 = sel4AM)     /\ (u = usm11)         /\
+          (k1 = kim21)        /\ (k2 = kim21)))      /\
+
+     (appraise _  = F)`;
+
+
+val _ = type_abbrev ("cache",``:(place, bool # num # bool) balanced_map``);
+
+val is_accepted_def = Define
+    `is_accepted c p = case (balanced_map$lookup place_cmp p c)
+                        of NONE => F
+                         | SOME (a,_,_) => a`;
+
+val is_time_expired_def = Define
+    `is_time_expired c p curr_time =
+         case (balanced_map$lookup place_cmp p c)
+          of NONE => F
+           | SOME (_,t,_) => curr_time < t`;
+
+val is_waiting_def = Define
+    `is_waiting c p = case (balanced_map$lookup place_cmp p c)
+                       of NONE => F
+                        | SOME (_,_,w) => w`;
+
+val check_cache_before_req_def = Define
+    `check_cache_before_req c p curr_t =
+         is_accepted c p /\ is_time_expired c p curr_t /\ ~(is_waiting c p)`;
+
+val update_cache_def = Define
+    `update_cache c p curr_t a w =
+          balanced_map$insert place_cmp p (a,curr_t + 1800,w) c`;
+
+val _ = Hol_datatype `
+    state_references = <| cache_ref : cache |>`;
+
+val config = global_state_config |> with_state ``:state_references``
+                                 |> with_refs [("cache_ref", ``balanced_map$empty : cache``)];
+
+val check_cache_or_request_def = Define `
+    check_cache_or_request msg time =
+        let place = userAM;
+        in do
+            c <- get_cache_ref;
+            if (check_cache_before_req c place time)
+            then return T
+            else (do set_cache_ref (update_cache c place time F T); return F od)
+           od`;
+
+val response_and_appraise_def = Define `
+    response_and_appraise msg time attn_res =
+        let place = userAM;
+            acc = appraise attn_res
+           in do
+               c <- get_cache_ref;
+               if is_waiting c place then set_cache_ref (update_cache c place time acc F) else set_cache_ref c;
+               return (acc /\ is_waiting c place)
+              od`;
+
+(* val _ = translation_extends "basisProg"; *)
+val res = translate empty_def;
+val res = start_translation config;
+
+val res = translate num_cmp_def;
+val res = translate w322n_def;
+val res = translate place_cmp_def;
+
+(* translated in basis library as well, but unable to merge a.t.m. *)
+val res = translate lookup_def;
+val res = translate delta_def;
+val res = translate singleton_def;
+val res = translate ratio_def;
+val res = translate size_def;
+val res = translate balanceL_def;
+val res = translate balanceR_def;
+val res = translate insert_def;
+
+val res = ml_prog_update (open_module "Appraiser");
+
+val res = translate sel4AM_def;
+val res = translate platformAM_def;
+val res = translate userAM_def;
+
+val res = translate usm11_def;
+val res = translate kim11_def;
+
+val res = translate expected_bs1_def;
+val res = translate expected_bs2_def;
+val res = translate expected_bs3_def;
+val res = translate expected_bs4_def;
+val res = translate expected_bs5_def;
+val res = translate expected_bs6_def;
+
+val res = translate appraise_def;
+val res = translate attestation_cmd_def;
+
+val res = translate is_accepted_def;
+val res = translate is_time_expired_def;
+val res = translate is_waiting_def;
+
+val res = translate check_cache_before_req_def;
+val res = translate update_cache_def;
+
+val res = m_translate check_cache_or_request_def;
+val res = m_translate response_and_appraise_def;
+
+val res = ml_prog_update (close_module NONE)
+
+val _ = export_theory();
